(wip) add open data

Core/Term/Definition.lean
@@ -6,23 +6,24 @@ open LeanSubst
 open Lilac
 
 namespace Core
+
 inductive Ctor0Variant : Type where
-| zero
+| fail
 | refl (A : Ty)
 
+inductive SpCtorVariant : Type where
+| openm
+| odata
+| cdata
+
 inductive Ctor1Variant : Type where
-| sym
 | prj (n : Nat)
 | appt (a : Ty)
 
 inductive Ctor2Variant : Type where
 | app (b : BaseKind)
 | cast
-| seq
-| appc
 | apptc
-| arrowc
-| choice
 
 inductive TyBindVariant : Type where
 | lamt
@@ -36,30 +37,32 @@ def Pattern.bind : Pattern m -> Nat
 
 inductive Term : Type where
 | var : Nat -> Term
-| global : String -> Term
-| dctor n : String -> List Ty -> Fun.Vec Term n -> Term
+| defn : String -> Term
+| spctor : SpCtorVariant -> String -> List Ty -> Fun.Vec Term n -> Term
 | ctor0 : Ctor0Variant -> Term
 | ctor1 : Ctor1Variant -> Term -> Term
 | ctor2 : Ctor2Variant -> Term -> Term -> Term
 | tbind : TyBindVariant -> Kind -> Term -> Term
 | lam : Ty -> Term -> Term
-| guard : Term -> Term -> Term -> Term
 | cast : Ty -> Term -> Term -> Term
 | mtch m n : Fun.Vec Term m -> Fun.Vec (Pattern m) n -> Fun.Vec Term n -> Term
 
 def Constructor := String × List Ty × List Term
 
 prefix:max "#" => Term.var
-prefix:max "g#" => Term.global
+prefix:max "d#" => Term.defn
+
+-- spctor notation
+notation "ctor!" => Term.spctor SpCtorVariant.cdata
+notation "inst!" => Term.spctor SpCtorVariant.odata
+notation "openm!" => Term.spctor SpCtorVariant.openm
 
 -- ctor0 notation
-notation "`0" => Term.ctor0 Ctor0Variant.zero
+notation "fail!" => Term.ctor0 Ctor0Variant.fail
 notation "refl! " A => Term.ctor0 (Ctor0Variant.refl A)
 
 -- ctor1 notation
-prefix:max "sym!" => Term.ctor1 Ctor1Variant.sym
 notation "prj[" n "]" t => Term.ctor1 (Ctor1Variant.prj n) t
-notation "snd!" t => Term.ctor1 Ctor1Variant.snd t
 notation f " •[" a "]" => Term.ctor1 (Ctor1Variant.appt a) f
 
 -- ctor2 notation
@@ -67,11 +70,7 @@ notation:70 f " •(" b ") " a:70 => Term.ctor2 (Ctor2Variant.app b) f a
 notation:70 f " • " a:70 => Term.ctor2 (Ctor2Variant.app BaseKind.closed) f a
 notation f " ∘[" a "]" => Term.ctor2 (Ctor2Variant.app BaseKind.open) f a
 notation t " ▹ " c => Term.ctor2 Ctor2Variant.cast t c
-notation t1 " `; " t2 => Term.ctor2 Ctor2Variant.seq t1 t2
-notation f " •c " a => Term.ctor2 Ctor2Variant.appc f a
 notation f " •c[" a "]" => Term.ctor2 Ctor2Variant.apptc f a
-notation A " -c> " B => Term.ctor2 Ctor2Variant.arrowc A B
-notation t1 " `+ " t2 => Term.ctor2 Ctor2Variant.choice t1 t2
 
 -- bind notation
 notation "Λ[" K "]" t => Term.tbind TyBindVariant.lamt K t
@@ -81,8 +80,8 @@ notation "∀c[" K "]" P => Term.tbind TyBindVariant.allc K P
 @[simp]
 def Term.size : Term -> Nat
 | var _ => 0
-| global _ => 0
-| dctor _ _ _ t2 =>
+| defn _ => 0
+| spctor _ _ _ t2 =>
   let t2' : Fun.Vec _ _ := size <$> t2
   Vec.sum t2'.to + 1
 | ctor0 _ => 0
@@ -90,7 +89,6 @@ def Term.size : Term -> Nat
 | ctor2 _ t1 t2 => size t1 + size t2 + 1
 | tbind _ _ t => size t + 1
 | lam _ t => size t + 1
-| guard t1 t2 t3 => size t1 + size t2 + size t3 + 1
 | cast _ t1 t2 => size t1 + size t2 + 1
 | mtch _ _ t1 _ t3 =>
   let t1' : Fun.Vec _ _ := size <$> t1
@@ -103,11 +101,10 @@ instance instSizeOf_Term : SizeOf Term where
 
 protected def Term.repr (p : Nat) : (a : Term) -> Std.Format
 | .var n => "#" ++ Nat.repr n
-| .global n => "g#" ++ n
-| dctor _ _ _ _ => "don't care"
+| .defn n => "d#" ++ n
+| spctor _ _ _ _ => "don't care"
 | .ctor0 (.refl t) => Std.Format.paren ("refl! " ++ Ty.repr max_prec t)
-| .ctor0 .zero => "`0"
-| .ctor1 .sym t => "(sym! " ++ Term.repr p t ++ ")"
+| .ctor0 .fail => "fail!"
 | .ctor1 (.prj n) t => "(prj! " ++ Nat.repr n ++ " " ++ Term.repr p t ++ ")"
 | .ctor1 (.appt τ) t => Repr.addAppParen (Term.repr max_prec t ++ " •[" ++ repr τ ++ "]") p
 | .ctor2 (.app .closed) t1 t2 =>
@@ -116,19 +113,9 @@ protected def Term.repr (p : Nat) : (a : Term) -> Std.Format
   Repr.addAppParen (Term.repr max_prec t1 ++ " ∘" ++ Std.Format.sbracket (Term.repr p t2)) p
 | .ctor2 .cast t1 t2 =>
   Repr.addAppParen ((Term.repr max_prec t1 ++ " • " ++ Term.repr p t2)) p
-| .ctor2 .seq t1 t2 =>
-  Repr.addAppParen (Term.repr max_prec t1 ++ "`;" ++
-  Std.Format.line ++ Term.repr p t2) p
-| .ctor2 .appc t1 t2 =>
-  Repr.addAppParen (Term.repr max_prec t1 ++ " •c " ++
-  Std.Format.line ++ Term.repr max_prec t2) p
 | .ctor2 .apptc t1 t2 =>
   Repr.addAppParen (Term.repr max_prec t1 ++
   Std.Format.line ++ " •c" ++ Std.Format.sbracket (Term.repr p t2)) p
-| .ctor2 .arrowc t1 t2 =>
-  Repr.addAppParen (Term.repr max_prec t1 ++ " -c> " ++ Term.repr p t2) p
-| .ctor2 .choice t1 t2 =>
-  Repr.addAppParen (Term.repr max_prec t1 ++ " `+ " ++ Term.repr max_prec t2) p
 | .tbind .lamt K t =>
   Repr.addAppParen ("Λ" ++ Std.Format.sbracket (repr K) ++ " " ++ Term.repr max_prec t) p
 | .tbind .allc K t =>
@@ -145,9 +132,6 @@ protected def Term.repr (p : Nat) : (a : Term) -> Std.Format
   --   ++ css
   --   ++ (Std.Format.nest 4 <| Std.Format.line ++ " _ => " ++ Term.repr p allc)
   --   )
-| .guard pat s t =>
-  Std.Format.nest 4 <| ("guard " ++ Term.repr p pat ++ " ← " ++ Term.repr p s) ++
-  Std.Format.line ++ Term.repr p t
 
 @[simp]
 instance instRepr_Term : Repr Term where
