Core/Term/Variant.lean
@@ -4,70 +4,66 @@ import Core.Term.Definition
 open LeanSubst
 namespace Core
 
-def Term.not_choice : Term -> Bool
-| ctor2 .choice _ _ => false
-| _ => true
+-- inductive Variant : Type where
+-- | ctor0 : Ctor0Variant -> Variant
+-- | ctor1 : Ctor1Variant -> Variant
+-- | ctor2 : Ctor2Variant -> Variant
+-- | tbind : TyBindVariant -> Variant
+-- | lam : Variant
+-- | guard : Variant
+-- | mtch : Variant
 
-inductive Variant : Type where
-| ctor0 : Ctor0Variant -> Variant
-| ctor1 : Ctor1Variant -> Variant
-| ctor2 : Ctor2Variant -> Variant
-| tbind : TyBindVariant -> Variant
-| lam : Variant
-| guard : Variant
-| mtch : Variant
+-- @[coe]
+-- def Variant.from_ctor0 (c : Ctor0Variant) : Variant := ctor0 c
 
-@[coe]
-def Variant.from_ctor0 (c : Ctor0Variant) : Variant := ctor0 c
+-- instance : Coe Ctor0Variant Variant where
+--   coe := Variant.from_ctor0
 
-instance : Coe Ctor0Variant Variant where
-  coe := Variant.from_ctor0
+-- @[coe]
+-- def Variant.from_ctor1 (c : Ctor1Variant) : Variant := ctor1 c
 
-@[coe]
-def Variant.from_ctor1 (c : Ctor1Variant) : Variant := ctor1 c
+-- instance : Coe Ctor1Variant Variant where
+--   coe := Variant.from_ctor1
 
-instance : Coe Ctor1Variant Variant where
-  coe := Variant.from_ctor1
+-- @[coe]
+-- def Variant.from_ctor2 (c : Ctor2Variant) : Variant := ctor2 c
 
-@[coe]
-def Variant.from_ctor2 (c : Ctor2Variant) : Variant := ctor2 c
+-- instance : Coe Ctor2Variant Variant where
+--   coe := Variant.from_ctor2
 
-instance : Coe Ctor2Variant Variant where
-  coe := Variant.from_ctor2
+-- @[coe]
+-- def Variant.from_tbind (c : TyBindVariant) : Variant := tbind c
 
-@[coe]
-def Variant.from_tbind (c : TyBindVariant) : Variant := tbind c
+-- instance : Coe TyBindVariant Variant where
+--   coe := Variant.from_tbind
 
-instance : Coe TyBindVariant Variant where
-  coe := Variant.from_tbind
-
-inductive VariantMissing : List Variant -> Term -> Prop where
-| var : VariantMissing vs #x
-| global : VariantMissing vs g#x
-| ctor0 {c : Ctor0Variant} :
-  ↑c ∉ vs ->
-  VariantMissing vs (.ctor0 c)
-| ctor1 {c : Ctor1Variant} :
-  ↑c ∉ vs ->
-  VariantMissing vs t ->
-  VariantMissing vs (.ctor1 c t)
-| ctor2 {c : Ctor2Variant} :
-  ↑c ∉ vs ->
-  VariantMissing vs t1 ->
-  VariantMissing vs t2 ->
-  VariantMissing vs (.ctor2 c t1 t2)
-| tbind {c : TyBindVariant} :
-  ↑c ∉ vs ->
-  VariantMissing vs t ->
-  VariantMissing vs (.tbind c K t)
-| lam :
-  VariantMissing vs t ->
-  VariantMissing vs (.lam A t)
-| guard :
-  VariantMissing vs t1 ->
-  VariantMissing vs t2 ->
-  VariantMissing vs t3 ->
-  VariantMissing vs (.guard t1 t2 t3)
+-- inductive VariantMissing : List Variant -> Term -> Prop where
+-- | var : VariantMissing vs #x
+-- | global : VariantMissing vs g#x
+-- | ctor0 {c : Ctor0Variant} :
+--   ↑c ∉ vs ->
+--   VariantMissing vs (.ctor0 c)
+-- | ctor1 {c : Ctor1Variant} :
+--   ↑c ∉ vs ->
+--   VariantMissing vs t ->
+--   VariantMissing vs (.ctor1 c t)
+-- | ctor2 {c : Ctor2Variant} :
+--   ↑c ∉ vs ->
+--   VariantMissing vs t1 ->
+--   VariantMissing vs t2 ->
+--   VariantMissing vs (.ctor2 c t1 t2)
+-- | tbind {c : TyBindVariant} :
+--   ↑c ∉ vs ->
+--   VariantMissing vs t ->
+--   VariantMissing vs (.tbind c K t)
+-- | lam :
+--   VariantMissing vs t ->
+--   VariantMissing vs (.lam A t)
+-- | guard :
+--   VariantMissing vs t1 ->
+--   VariantMissing vs t2 ->
+--   VariantMissing vs t3 ->
+--   VariantMissing vs (.guard t1 t2 t3)
 -- | mtch {ps : Vect n _} :
 --   VariantMissing vs t ->
 --   (∀ i, VariantMissing vs (ps i)) ->
